\documentclass[a4paper]{ctexart}
\usepackage{lmodern}
\usepackage{amsmath}
\usepackage{amsthm}
\usepackage[textwidth=14.5cm]{geometry}
\usepackage{blindtext}
\parindent=0pt

\begin{document}
\begin{sloppypar}
    \begin{proof}
        已知:
        $$
            T(n) =
            \left\{
            \begin{aligned}
                 & O(1)                   & n =1  \\
                 & kT(\frac{n}{m}) + f(n) & n > 1
            \end{aligned}
            \right.
        $$
        当$n > 1$时, 有
        \begin{equation}
            \begin{aligned}
                \nonumber
                T(n) & = kT(\frac{n}{m}) + f(n)                                                              \\
                     & = k[kT(\frac{n}{m^2}) + f(\frac{n}{m})] +f(n)                                         \\
                     & = k^2T(\frac{n}{m^2}) + kf(\frac{n}{m}) + f(n)                                        \\
                     & = k^2[kT(\frac{n}{m^3}) + f(\frac{n}{m^2})] + kf(\frac{n}{m}) + f(n)                  \\
                     & = k^3T(\frac{n}{m^3}) + k^2f(\frac{n}{m^2}) + kf(\frac{n}{m}) + f(n)                  \\
                     & \;\;\vdots                                                                            \\
                     & = k^xT(\frac{n}{m^x}) + k^{x-1}f(\frac{n}{m^{x-1}}) + \cdots + kf(\frac{n}{m}) + f(n) \\
            \end{aligned}
        \end{equation}
        令$\frac{n}{m^x} = 1$, 则有$x = \log_{m}{n}$\\
        \begin{equation}
            \begin{aligned}
                \nonumber
                T(n) & = k^{\log_{m}{n}}T(1) + k^{\log_{m}{n}-1}f(\frac{n}{m^{\log_{m}{n}-1}}) + \cdots + kf(\frac{n}{m}) + f(n) \\
                     & = k^{\log_{m}{n}}O(1) + \sum_{i=0}^{\log_{m}{n}-1}k^if(\frac{n}{m^i})                                     \\
                     & = k^{\frac{\log_{k}{n}}{\log_{k}{m}}}O(1) + \sum_{i=0}^{\log_{m}{n}-1}k^if(\frac{n}{m^i})                 \\
                     & = k^{\log_{k}{n}\log_{m}{k}}O(1) + \sum_{i=0}^{\log_{m}{n}-1}k^if(\frac{n}{m^i})                          \\
                     & = n^{\log_{m}{k}}O(1) + \sum_{i=0}^{\log_{m}{n}-1}k^if(\frac{n}{m^i})                                     \\
            \end{aligned}
        \end{equation}
    \end{proof}
\end{sloppypar}
\end{document}
